examples/stateful_bignum/subtraction_st.fst
@@ -1,4 +1,9 @@
-module Substraction
+(*--build-config
+  options:--admit_fsi FStar.Seq --admit_fsi FStar.Set --verify_module Subtraction --z3timeout 150;
+  other-files:classical.fst ext.fst set.fsi seq.fsi seqproperties.fst heap.fst st.fst all.fst arr.fst ghost.fst axiomatic.fst intlib.fst limb.fst bigint_st.fst eval_st.fst;
+  --*)
+
+module Subtraction
 
 open IntLib
 open Limb
@@ -10,13 +15,13 @@ open FStar.Heap
 open Bigint
 
 (* 
-   Auxiliary substraction function. 
+   Auxiliary subtraction function. 
    Takes two input arrays, the current index for the computation and the temporary result 
  *)
 
-(* Auxiliary substraction function putting the result in the first operand *)
+(* Auxiliary subtraction function putting the result in the first operand *)
 (* Code, not tailrecursive, proof without witness *)
-val substraction:
+val subtraction:
   a:bigint -> a_idx:nat ->  b:bigint -> b_idx:nat -> len:nat ->
   ST unit
     (requires (fun h -> 
@@ -61,31 +66,31 @@ val substraction:
 		    getSize h1 a i = getSize h0 a i)
  
 ))
-let rec substraction a a_idx b b_idx len =
+let rec subtraction a a_idx b b_idx len =
   match len with
   | 0 -> ()
   |  _ -> 
-      let h0 = erase (ST.get()) in
-      substraction a a_idx b b_idx (len-1);
+      let h0 = (ST.get()) in
+      subtraction a a_idx b b_idx (len-1);
       let h1 =
-	erase (ST.get ()) in
+	(ST.get ()) in
       let ai = Bigint.get a (a_idx+len-1) in
       let size_ai =
-	erase (getSize h1 a (a_idx+len-1)) in
+	(getSize h1 a (a_idx+len-1)) in
       let bi = Bigint.get b (b_idx+len-1) in
       let size_bi = 
-	erase (getSize h1 b (b_idx+len-1)) in
+	(getSize h1 b (b_idx+len-1)) in
       let v = Limb.sub size_ai ai size_bi bi in
-      erase (
+      (
 	  order_n_bits v (max size_ai size_bi + 1) (wordSize a - 1));
-      let (t:tint (wordSize a)) = mk_tint a (erase (max size_ai size_bi + 1))  v in
-      let h1 = erase (ST.get()) in
+      let (t:tint (wordSize a)) = mk_tint a ((max size_ai size_bi + 1))  v in
+      let h1 = (ST.get()) in
       updateBigint a (a_idx+len-1) t
 
 
 (* Code *)
-(* Tail recursive version of the substraction *)
-val substraction_tr:
+(* Tail recursive version of the subtraction *)
+val subtraction_tr:
   ghost_a:seq (tint ocaml63) -> a:bigint -> a_idx:nat ->  b:bigint -> b_idx:nat -> len:nat -> ctr:nat ->
   ST unit
     (requires (fun h -> 
@@ -134,27 +139,27 @@ val substraction_tr:
    
 ))
 
-let rec substraction_tr ghost_a a a_idx b b_idx len ctr =
+let rec subtraction_tr ghost_a a a_idx b b_idx len ctr =
   match len - ctr with
   | 0 -> ()
   | _ -> 
       let i = ctr in
       let h1 =
-	erase (ST.get ()) in
+	(ST.get ()) in
       let ai = Bigint.get a (a_idx+i) in
       let size_ai =
-	erase (getSize h1 a (a_idx+i)) in
+	(getSize h1 a (a_idx+i)) in
       let bi = Bigint.get b (b_idx+i) in
       let size_bi = 
-	erase (getSize h1 b (b_idx+i)) in
+	(getSize h1 b (b_idx+i)) in
       let v = Limb.sub size_ai ai size_bi bi in
-      let (t:tint (wordSize a)) = mk_tint a (erase (max size_ai size_bi + 1))  v in
+      let (t:tint (wordSize a)) = mk_tint a ((max size_ai size_bi + 1))  v in
       updateBigint a (a_idx+i) t;
-      substraction_tr ghost_a a a_idx b b_idx len (ctr+1);
+      subtraction_tr ghost_a a a_idx b b_idx len (ctr+1);
       ()
 
 
-val substraction_lemma_aux:
+val subtraction_lemma_aux:
   h0:heap ->
   h1:heap ->
   a:bigint{ (inHeap h0 a) 
@@ -172,12 +177,12 @@ val substraction_lemma_aux:
     (requires ( (eval h0 a (len-1) - eval h0 b (len-1) = eval h1 a (len-1))
 		/\ (getValue h1 a (len-1) = getValue h0 a (len-1) - getValue h0 b (len-1)) ) )
     (ensures (eval h0 a len - eval h0 b len = eval h1 a len))
-let substraction_lemma_aux h0 h1 a b len =
-  erase (
+let subtraction_lemma_aux h0 h1 a b len =
+  (
       distributivity_sub_right (pow2 (bitweight (Bigint63.t a) (len-1))) (getValue h0 a (len-1))  (getValue h0 b (len-1))
     )
 
-val substraction_lemma:
+val subtraction_lemma:
   h0:heap ->
   h1:heap ->
   a:bigint{ (inHeap h0 a) 
@@ -194,15 +199,15 @@ val substraction_lemma:
   Lemma
     (requires (True))
     (ensures ( eval h0 a len - eval h0 b len = eval h1 a len ))
-let rec substraction_lemma h0 h1 a b len =
-  erase (
+let rec subtraction_lemma h0 h1 a b len =
+  (
       match len with
       | 0 -> ()
-      | _ -> substraction_lemma h0 h1 a b (len-1);
-	     substraction_lemma_aux h0 h1 a b len
+      | _ -> subtraction_lemma h0 h1 a b (len-1);
+	     subtraction_lemma_aux h0 h1 a b len
     )
 
-val substraction_max_value_lemma:
+val subtraction_max_value_lemma:
   h0:heap -> 
   h1:heap -> 
   a:bigint{ (inHeap h0 a)
@@ -217,9 +222,9 @@ val substraction_max_value_lemma:
   Lemma
     (requires (True))
     (ensures (maxValue h1 c <= maxValue h0 a + maxValue h0 b))
-let substraction_max_value_lemma h0 h1 a b c = ()
+let subtraction_max_value_lemma h0 h1 a b c = ()
   
-val substraction_max_size_lemma:
+val subtraction_max_size_lemma:
   h0:heap -> 
   h1:heap -> 
   a:bigint{ (inHeap h0 a) } -> 
@@ -232,7 +237,7 @@ val substraction_max_size_lemma:
   Lemma
     (requires (True))
     (ensures (maxSize h1 c <= max (maxSize h0 a) (maxSize h0 b) + 1))
-let substraction_max_size_lemma h0 h1 a b c = ()
+let subtraction_max_size_lemma h0 h1 a b c = ()
 
 val max_value_lemma: h:heap -> a:bigint{ inHeap h a } -> m:nat ->
 		     Lemma 
@@ -243,7 +248,7 @@ let max_value_lemma h a m = ()
 val abs_lemma: unit -> Lemma (ensures (forall a b. abs (a + b) <= abs a + abs b))
 let abs_lemma () = () 
 
-val substraction_max_value_lemma_extended:
+val subtraction_max_value_lemma_extended:
   h0:heap -> 
   h1:heap -> 
   a:bigint{ (inHeap h0 a) } -> 
@@ -258,8 +263,8 @@ val substraction_max_value_lemma_extended:
 	       /\ (forall (i:nat). ( i < getLength h1 c /\ (i < idx \/ i >= idx + len))
 		   ==> getValue h1 c i = getValue h0 a i)))
     (ensures (maxValue h1 c <= maxValue h0 a + maxValue h0 b))
-let substraction_max_value_lemma_extended h0 h1 a b c idx len = 
-  erase (
+let subtraction_max_value_lemma_extended h0 h1 a b c idx len = 
+  (
     cut ( forall (i:nat). (i < getLength h1 c /\ (i < idx \/ i >= idx + len))
 	  ==> (getValue h1 c i = getValue h0 a i /\ abs (getValue h1 c i) <= maxValue h0 a + maxValue h0 b));
     cut ( forall (i:nat). (i < getLength h1 c /\ (i < idx \/ i >= idx + len)) 
@@ -278,7 +283,7 @@ let substraction_max_value_lemma_extended h0 h1 a b c idx len =
     ()
   )
     
-val substraction_max_size_lemma_extended:
+val subtraction_max_size_lemma_extended:
   h0:heap -> 
   h1:heap -> 
   a:bigint{ (inHeap h0 a) } -> 
@@ -293,7 +298,7 @@ val substraction_max_size_lemma_extended:
 	       /\ (forall (i:nat). ( i < getLength h1 c /\ (i < idx \/ i >= idx + len))
 		   ==> getSize h1 c i = getSize h0 a i)))
     (ensures (maxSize h1 c <= max (maxSize h0 a) (maxSize h0 b) + 1))
-let substraction_max_size_lemma_extended h0 h1 a b c idx len = 
+let subtraction_max_size_lemma_extended h0 h1 a b c idx len = 
   cut ( forall (i:nat). (i < getLength h1 c /\ (i < idx \/ i >= idx + len))
 	==> (getSize h1 c i = getSize h0 a i /\ getSize h1 c i <= max (maxSize h0 a) (maxSize h0 b) + 1) );
   cut ( forall (i:nat). (i < getLength h1 c /\ (i < idx \/ i >= idx + len)) 
@@ -311,7 +316,7 @@ let substraction_max_size_lemma_extended h0 h1 a b c idx len =
   ()
 
 
-val substraction_with_lemma:
+val subtraction_with_lemma:
   a:bigint -> b:bigint -> len:nat ->
   ST unit
     (requires (fun h -> 
@@ -340,13 +345,13 @@ val substraction_with_lemma:
       /\ (Seq.length (sel h1 (Bigint63.data b)) >= len)
       /\ (eval h1 a len = eval h0 a len - eval h0 b len)
     ))
-let substraction_with_lemma a b len =
+let subtraction_with_lemma a b len =
   let h0 =
-    erase (ST.get()) in
-  substraction_tr (erase (Array.to_seq (Bigint63.data a))) a 0 b 0 len 0;
-  erase (
+    (ST.get()) in
+  subtraction_tr ((Array.to_seq (Bigint63.data a))) a 0 b 0 len 0;
+  (
       let h1 = ST.get() in      
-      substraction_lemma h0 h1 a b len;
-      substraction_max_value_lemma_extended h0 h1 a b a 0 len;
-      substraction_max_size_lemma_extended h0 h1 a b a 0 len
+      subtraction_lemma h0 h1 a b len;
+      subtraction_max_value_lemma_extended h0 h1 a b a 0 len;
+      subtraction_max_size_lemma_extended h0 h1 a b a 0 len
     )
